src/certigrad/aevb/grads_correct.lean
@@ -8,8 +8,8 @@ applied to the naive variational encoder.
 -/
 import .util .naive ..prove_model_ok ..pre .sub_exp
 
-set_option class.instance_max_depth 1000000
-set_option max_memory 10000000
+set_option class.instance_max_depth 100000
+set_option max_memory 100000
 set_option pp.max_depth 100000
 
 namespace certigrad
@@ -78,9 +78,11 @@ end
 lemma g_final_grads_exist_at_he : grads_exist_at g^.nodes fdict (ID.str label.W_encode, [a^.ne, a^.n_in]) := sorry -- by cgsimp
 -- TODO(dhs): I don't know if this works or not, it takes freaking forever
 
+set_option trace.simplify.rewrite true
+
 lemma g_final_is_gintegrable_he :
   is_gintegrable (λ m, ⟦compute_grad_slow g^.costs g^.nodes m (ID.str label.W_encode, [a^.ne, a^.n_in])⟧)
-                 fdict g^.nodes dvec.head := sorry -- by cgsimp
+                 fdict g^.nodes dvec.head := by cgsimp >> prove_is_mvn_integrable
 -- TODO(dhs): crashes my machine, not sure if it just the type-checking
 
 lemma g_final_diff_under_int_hem :
