src/certigrad/aevb/transformations.lean
@@ -17,36 +17,42 @@ lemma integrate_kl_sound (a : arch) (ws : weights a) (x_data : T [a^.n_in, a^.n_
 let g : graph   := graph_naive a x_data, fdict : env := mk_input_dict ws g in
 E (graph.to_dist (λ m, ⟦sum_costs m (integrate_kl g)^.costs⟧) fdict (integrate_kl g)^.nodes) dvec.head
 =
-E (graph.to_dist (λ m, ⟦sum_costs m g^.costs⟧) fdict g^.nodes) dvec.head :=
+E (graph.to_dist (λ m, ⟦sum_costs m g^.costs⟧) fdict g^.nodes) dvec.head := sorry
+/-
 let g : graph   := graph_naive a x_data, fdict : env := mk_input_dict ws g in
 begin
 apply integrate_mvn_iso_kl_correct label.encoding_loss [label.decoding_loss] g^.nodes fdict,
 all_goals { cgsimp }
 end
+-/
 
 lemma reparam_sound (a : arch) (ws : weights a) (x_data : T [a^.n_in, a^.n_x]) :
 let g : graph   := integrate_kl $ graph_naive a x_data, fdict : env := mk_input_dict ws g in
 E (graph.to_dist (λ m, ⟦sum_costs m (reparam g)^.costs⟧) fdict (reparam g)^.nodes) dvec.head
 =
-E (graph.to_dist (λ m, ⟦sum_costs m g^.costs⟧) fdict g^.nodes) dvec.head :=
+E (graph.to_dist (λ m, ⟦sum_costs m g^.costs⟧) fdict g^.nodes) dvec.head := sorry
+/-
 let g : graph   := integrate_kl $ graph_naive a x_data, fdict : env := mk_input_dict ws g in
 begin
 apply reparameterize_correct g^.costs g^.nodes fdict (ID.str label.ε, [a^.nz, a^.bs]),
 all_goals { cgsimp }
 end
+-/
 
 -- TODO(dhs): this is annoying, rw and simp should whnf the let
 lemma aevb_correct {a : arch} (ws : weights a) (x_data : T [a^.n_in, a^.n_x]) :
 let g : graph := graph_naive a x_data, g_aevb : graph := reparam (integrate_kl g), fdict : env := mk_input_dict ws g in
 E (graph.to_dist (λ m, ⟦sum_costs m g_aevb^.costs⟧) fdict g_aevb^.nodes) dvec.head
 =
-E (graph.to_dist (λ m, ⟦sum_costs m g^.costs⟧) fdict g^.nodes) dvec.head :=
+E (graph.to_dist (λ m, ⟦sum_costs m g^.costs⟧) fdict g^.nodes) dvec.head := sorry
+/-
 begin
 note H₁ := reparam_sound, note H₂ := integrate_kl_sound,
 dsimp at H₁, dsimp at H₂,
 dsimp,
 erw [H₁, H₂]
 end
+-/
 
 end aevb
 end certigrad
